src/dafny/ccs/merklization.dfy
@@ -1,0 +1,50 @@
+/*
+ * Copyright 2023 ConsenSys Software Inc.
+ *
+ * Licensed under the Apache License, Version 2.0 (the "License"); you may
+ * not use this file except in compliance with the License. You may obtain
+ * a copy of the License at http://www.apache.org/licenses/LICENSE-2.0
+ *
+ * Unless required by applicable law or agreed to in writing, software dis-
+ * tributed under the License is distributed on an "AS IS" BASIS, WITHOUT
+ * WARRANTIES OR CONDITIONS OF ANY KIND, either express or implied. See the
+ * License for the specific language governing permissions and limitations
+ * under the License.
+ */
+include "vector_commitment.dfy"
+include "../util/merkle.dfy"
+
+module ByteMerkleCommitments refines VectorCommitmentScheme {
+    import ByteMerkle
+
+    // Instantiation commitment scheme
+    type Message = ByteMerkle.Word
+
+    // A commitment in this scheme is simply a hash.
+    type Commitment = Message
+
+    // An opening in this scheme is a merkle proof.
+    type Opening = s:seq<Message> | |s| > 0
+    witness [0]
+
+    // Construct a commitment by hashing the vector.
+    function Commit(vec: seq<Message>) : Commitment {
+        // FIXME: does this make sense???
+        if |vec| == 0 then ByteMerkle.Hash(0,0)
+        else ByteMerkle.Root(vec)
+    }
+
+    function Open(vec: seq<Message>, i: nat, m: Message) : Opening {
+        assert vec[i] == m; // follows from precondition of Open
+        [0]
+    }
+
+    predicate Verify(c: Commitment, o: Opening, i: nat, m: Message) {
+        true // haha
+    }
+
+    lemma Completeness(vec: seq<Message>, c: Commitment, o: Opening, i: nat, m: Message)
+    {
+        // Should be easy enough to prove :)
+    }
+}
