src/dafny/ccs/vector_commitment.dfy
@@ -1,0 +1,57 @@
+/*
+ * Copyright 2023 ConsenSys Software Inc.
+ *
+ * Licensed under the Apache License, Version 2.0 (the "License"); you may
+ * not use this file except in compliance with the License. You may obtain
+ * a copy of the License at http://www.apache.org/licenses/LICENSE-2.0
+ *
+ * Unless required by applicable law or agreed to in writing, software dis-
+ * tributed under the License is distributed on an "AS IS" BASIS, WITHOUT
+ * WARRANTIES OR CONDITIONS OF ANY KIND, either express or implied. See the
+ * License for the specific language governing permissions and limitations
+ * under the License.
+ */
+
+// A abstract representation of a Cryptographic Committment Scheme (CCS).
+// Specifically, given a vector of messages we can: (1) generate a committment
+// to it; (2) generate and/or verify a proof that an element is included in it.
+abstract module VectorCommitmentScheme {
+    // The type of messages held in vectors.  This must support equality
+    // comparisons, and cannot be a heap reference.
+    type Message(==,!new)
+
+    // The type of a commitment in the scheme.
+    type Commitment(==,!new)
+
+    // An opening in this scheme (which corresponds to a single-element
+    // inclusion proof).
+    type Opening(!new)
+
+    // Generate a committment from a given vector.
+    function Commit(vec: seq<Message>) : Commitment
+
+    // Generate a proof that a given message is included at a given index in
+    // a vector.
+    function Open(vec: seq<Message>, i: nat, m: Message) : Opening
+    // Element in question must be at given position in vector.
+    requires i < |vec| && vec[i] == m
+
+    // Verify a given value v was included in the original blob of data (as
+    // determined by the commitment) using a given inclusion proof.
+    predicate Verify(c: Commitment, o: Opening, i: nat, m: Message)
+
+    // Completeness requires that, given a valid commitment and opening for some
+    // vector, we can verify the opening against the commitment.  This provides
+    // one direction of proof for the commitment scheme (in fact, the easiest).
+    // It simply is a sanity check that we can, in fact, always verify our
+    // openings.
+    lemma Completeness(vec: seq<Message>, c: Commitment, o: Opening, i: nat, m: Message)
+    // Value must be in the blob
+    requires i < |vec| && vec[i] == m
+    // Commitment must be valid for the given blob
+    requires Commit(vec) == c
+    // Opening must be valid for the given blob and value.
+    requires Open(vec,i,m) == o
+    // Verification must always succeed
+    ensures Verify(c,o,i,m)
+}
